Weidenbach_Book/IsaSAT_Arena.thy
@@ -2280,4 +2280,5 @@ lemma MAX_LENGTH_SHORT_CLAUSE_hnr[sepref_fr_rules]:
   \<open>(uncurry0 (return 5), uncurry0 (RETURN MAX_LENGTH_SHORT_CLAUSE)) \<in> unit_assn\<^sup>k \<rightarrow>\<^sub>a uint64_nat_assn\<close>
   by sepref_to_hoare (sep_auto simp: uint64_nat_rel_def br_def)
 
+
 end
